theories/typing/mod_ty.v
@@ -86,6 +86,22 @@ Section typing.
   Global Instance mod_ty_sync {𝔄 𝔅} (f: 𝔄 → 𝔅) ty : Sync ty → Sync (<{f}> ty).
   Proof. move=> ??*/=. by do 3 f_equiv. Qed.
 
+  Lemma mod_ty_leak' {𝔄 𝔅} E L (f: 𝔄 → 𝔅) ty Φ :
+    Leak E L ty Φ → Leak E L (<{f}> ty) (λ b, ∃a, b = f a ∧ Φ a).
+  Proof.
+    move=> Lk > ?. iIntros "LFT PROPH E L (%&->& ty)".
+    iMod (Lk with "LFT PROPH E L ty") as "ToObs"; [done|].
+    iApply (step_fupdN_wand with "ToObs"). iIntros "!> >[Obs $] !>".
+    iApply proph_obs_impl; [|done]=>/= ??. by eexists _.
+  Qed.
+
+  Lemma mod_ty_leak {𝔄 𝔅} E L f g `{!@SemiIso 𝔄 𝔅 f g} ty Φ :
+    Leak E L ty Φ → Leak E L (<{f}> ty) (Φ ∘ g).
+  Proof.
+    move=> ?. eapply leak_impl; [by apply mod_ty_leak'|]=>/=
+    ?[?[/(f_equal g) + ?]]. by rewrite semi_iso'=> ->.
+  Qed.
+
   Lemma mod_ty_own {𝔄 𝔅} g f `{!@Iso 𝔄 𝔅 f g} ty vπ d tid vl :
     (<{f}> ty).(ty_own) vπ d tid vl ⊣⊢ ty.(ty_own) (g ∘ vπ) d tid vl.
   Proof. iSplit=>/=.
@@ -146,4 +162,6 @@ Section typing.
 
 End typing.
 
+Global Hint Resolve mod_ty_leak | 10 : lrust_typing.
+Global Hint Resolve mod_ty_leak' | 20 : lrust_typing.
 Global Hint Resolve mod_ty_subtype mod_ty_eqtype : lrust_typing.
